vale/code/arch/x64/interop/Fast_stdcalls.fsti
@@ -25,7 +25,7 @@ val add1
   (requires fun h ->
     adx_enabled /\ bmi2_enabled /\
     B.live h out /\ B.live h f1 /\
-    B.disjoint out f1)
+    (B.disjoint out f1 \/ out == f1))
   (ensures fun h0 c h1 ->
     B.live h1 out /\ B.live h1 f1 /\
     B.modifies (B.loc_buffer out) h0 h1 /\
@@ -39,7 +39,24 @@ val fadd
     (requires fun h -> 
       adx_enabled /\ bmi2_enabled /\
       B.live h f1 /\ B.live h f2 /\ B.live h out /\
-      B.disjoint out f1 /\ B.disjoint out f2 /\ B.disjoint f1 f2)
+      (B.disjoint out f1 \/ out == f1) /\ 
+      (B.disjoint out f2 \/ out == f2) /\ 
+      (B.disjoint f1 f2 \/ f1 == f2))
     (ensures  fun h0 _ h1 ->
       B.modifies (B.loc_buffer out) h0 h1 /\
       (as_nat out h1) % prime == (as_nat f1 h0 + as_nat f2 h0) % prime)
+
+val fsub
+  (out:u256)
+  (f1:u256)
+  (f2:u256)
+  : Stack unit
+    (requires fun h -> 
+      adx_enabled /\ bmi2_enabled /\
+      B.live h f1 /\ B.live h f2 /\ B.live h out /\
+      (B.disjoint out f1 \/ out == f1) /\ 
+      (B.disjoint out f2 \/ out == f2) /\ 
+      (B.disjoint f1 f2 \/ f1 == f2))
+    (ensures  fun h0 _ h1 ->
+      B.modifies (B.loc_buffer out) h0 h1 /\
+      (as_nat out h1) % prime == (as_nat f1 h0 - as_nat f2 h0) % prime)
